Added a bunch of nice notation

Bananas.thy
@@ -4,64 +4,82 @@ begin
 
 datatype type = 
   Unit
-| Prod type type
-| Sum type type
-| Func type type (infixr "\<rightarrow>" 80)
-| Mu funct
+| Prod type type (infixr "\<otimes>" 80)
+| Sum type type (infixr "\<oplus>" 80)
+| Func type type (infixr "\<rightarrow>" 70)
+| \<mu> funct
 and funct =
   Id
 | K type
 | ProdF funct funct
 | SumF funct funct
 
-primrec apply_functor :: "funct \<Rightarrow> type \<Rightarrow> type" where
-  "apply_functor Id t = t"
-| "apply_functor (K t') t = t'"
-| "apply_functor (ProdF f\<^sub>1 f\<^sub>2) t = Prod (apply_functor f\<^sub>1 t) (apply_functor f\<^sub>2 t)"
-| "apply_functor (SumF f\<^sub>1 f\<^sub>2) t = Sum (apply_functor f\<^sub>1 t) (apply_functor f\<^sub>2 t)"
+primrec apply_functor :: "funct \<Rightarrow> type \<Rightarrow> type" (infixr "\<star>" 80) where
+  "Id \<star> t = t"
+| "K t' \<star> t = t'"
+| "ProdF f\<^sub>1 f\<^sub>2 \<star> t = (f\<^sub>1 \<star> t) \<otimes> (f\<^sub>2 \<star> t)"
+| "SumF f\<^sub>1 f\<^sub>2 \<star> t = (f\<^sub>1 \<star> t) \<oplus> (f\<^sub>2 \<star> t)"
 
 datatype expr = 
-  Apply expr expr (infixl "\<star>" 80)
+  Apply expr expr (infixl "\<cdot>" 70)
 | UnitV
-| Pair expr expr | Fst | Snd
-| Inl expr | Inr expr | Case expr expr
-| Inj funct expr | Outj funct
+| PairV expr expr 
+| InlV expr
+| InrV expr
+
+| \<pi>\<^sub>1 
+| \<pi>\<^sub>2 
+| Tuple expr expr (infix "\<triangle>" 80)
+| \<iota>\<^sub>l 
+| \<iota>\<^sub>r 
+| Case expr expr (infix "\<nabla>" 80)
+| Inj funct expr 
+| Outj funct
 
 inductive typecheck :: "expr \<Rightarrow> type \<Rightarrow> bool" (infix "\<turnstile>" 60) where
-  tc_app [simp]: "e\<^sub>1 \<turnstile> t\<^sub>1 \<rightarrow> t\<^sub>2 \<Longrightarrow> e\<^sub>2 \<turnstile> t\<^sub>1 \<Longrightarrow> e\<^sub>1 \<star> e\<^sub>2 \<turnstile> t\<^sub>2"
+  tc_app [simp]: "e\<^sub>1 \<turnstile> t\<^sub>1 \<rightarrow> t\<^sub>2 \<Longrightarrow> e\<^sub>2 \<turnstile> t\<^sub>1 \<Longrightarrow> e\<^sub>1 \<cdot> e\<^sub>2 \<turnstile> t\<^sub>2"
 | tc_unit [simp]: "UnitV \<turnstile> Unit"
-| tc_pair [simp]: "e\<^sub>1 \<turnstile> t\<^sub>1 \<Longrightarrow> e\<^sub>2 \<turnstile> t\<^sub>2 \<Longrightarrow> Pair e\<^sub>1 e\<^sub>2 \<turnstile> Prod t\<^sub>1 t\<^sub>2"
-| tc_fst [simp]: "Fst \<turnstile> Prod t\<^sub>1 t\<^sub>2 \<rightarrow> t\<^sub>1"
-| tc_snd [simp]: "Snd \<turnstile> Prod t\<^sub>1 t\<^sub>2 \<rightarrow> t\<^sub>2"
-| tc_inl [simp]: "e \<turnstile> t\<^sub>1 \<Longrightarrow> Inl e \<turnstile> Sum t\<^sub>1 t\<^sub>2"
-| tc_inr [simp]: "e \<turnstile> t\<^sub>2 \<Longrightarrow> Inr e \<turnstile> Sum t\<^sub>1 t\<^sub>2"
-| tc_case [simp]: "e\<^sub>1 \<turnstile> t\<^sub>1 \<rightarrow> t\<^sub>3 \<Longrightarrow> e\<^sub>2 \<turnstile> t\<^sub>2 \<rightarrow> t\<^sub>3 \<Longrightarrow> Case e\<^sub>1 e\<^sub>2 \<turnstile> Sum t\<^sub>1 t\<^sub>2 \<rightarrow> t\<^sub>3"
-| tc_inj [simp]: "e \<turnstile> apply_functor f (Mu f) \<Longrightarrow> Inj f e \<turnstile> Mu f"
-| tc_outj [simp]: "Outj f \<turnstile> Mu f \<rightarrow> apply_functor f (Mu f)"
+| tc_pair [simp]: "e\<^sub>1 \<turnstile> t\<^sub>1 \<Longrightarrow> e\<^sub>2 \<turnstile> t\<^sub>2 \<Longrightarrow> PairV e\<^sub>1 e\<^sub>2 \<turnstile> t\<^sub>1 \<otimes> t\<^sub>2"
+| tc_inlv [simp]: "e \<turnstile> t\<^sub>1 \<Longrightarrow> InlV e \<turnstile> t\<^sub>1 \<oplus> t\<^sub>2"
+| tc_inrv [simp]: "e \<turnstile> t\<^sub>2 \<Longrightarrow> InrV e \<turnstile> t\<^sub>1 \<oplus> t\<^sub>2"
+| tc_fst [simp]: "\<pi>\<^sub>1 \<turnstile> t\<^sub>1 \<otimes> t\<^sub>2 \<rightarrow> t\<^sub>1"
+| tc_snd [simp]: "\<pi>\<^sub>2 \<turnstile> t\<^sub>1 \<otimes> t\<^sub>2 \<rightarrow> t\<^sub>2"
+| tc_tup [simp]: "f\<^sub>1 \<turnstile> t\<^sub>1 \<rightarrow> t\<^sub>2 \<Longrightarrow> f\<^sub>2 \<turnstile> t\<^sub>1 \<rightarrow> t\<^sub>3 \<Longrightarrow> f\<^sub>1 \<triangle> f\<^sub>2 \<turnstile> t\<^sub>1 \<rightarrow> t\<^sub>2 \<otimes> t\<^sub>3"
+| tc_inl [simp]: "\<iota>\<^sub>l \<turnstile> t\<^sub>1 \<rightarrow> t\<^sub>1 \<oplus> t\<^sub>2"
+| tc_inr [simp]: "\<iota>\<^sub>r \<turnstile> t\<^sub>2 \<rightarrow> t\<^sub>1 \<oplus> t\<^sub>2"
+| tc_case [simp]: "f\<^sub>l \<turnstile> t\<^sub>1 \<rightarrow> t\<^sub>3 \<Longrightarrow> f\<^sub>r \<turnstile> t\<^sub>2 \<rightarrow> t\<^sub>3 \<Longrightarrow> f\<^sub>l \<nabla> f\<^sub>r \<turnstile> t\<^sub>1 \<oplus> t\<^sub>2 \<rightarrow> t\<^sub>3"
+| tc_inj [simp]: "e \<turnstile> f \<star> \<mu> f \<Longrightarrow> Inj f e \<turnstile> \<mu> f"
+| tc_outj [simp]: "Outj f \<turnstile> \<mu> f \<rightarrow> f \<star> \<mu> f"
 
-inductive_cases [elim]: "e\<^sub>1 \<star> e\<^sub>2 \<turnstile> t"
+inductive_cases [elim]: "e\<^sub>1 \<cdot> e\<^sub>2 \<turnstile> t"
 inductive_cases [elim]: "UnitV \<turnstile> t"
-inductive_cases [elim]: "Pair e\<^sub>1 e\<^sub>2 \<turnstile> t"
-inductive_cases [elim]: "Fst \<turnstile> t"
-inductive_cases [elim]: "Snd \<turnstile> t"
-inductive_cases [elim]: "Inl e \<turnstile> t"
-inductive_cases [elim]: "Inr e \<turnstile> t"
-inductive_cases [elim]: "Case e\<^sub>1 e\<^sub>2 \<turnstile> t"
+inductive_cases [elim]: "PairV e\<^sub>1 e\<^sub>2 \<turnstile> t"
+inductive_cases [elim]: "InrV e \<turnstile> t"
+inductive_cases [elim]: "InlV e \<turnstile> t"
+inductive_cases [elim]: "\<pi>\<^sub>1 \<turnstile> t"
+inductive_cases [elim]: "\<pi>\<^sub>2 \<turnstile> t"
+inductive_cases [elim]: "f\<^sub>1 \<triangle> f\<^sub>2 \<turnstile> t"
+inductive_cases [elim]: "\<iota>\<^sub>l \<turnstile> t"
+inductive_cases [elim]: "\<iota>\<^sub>r \<turnstile> t"
+inductive_cases [elim]: "f\<^sub>l \<nabla> f\<^sub>r \<turnstile> t"
 inductive_cases [elim]: "Inj f e \<turnstile> t"
 inductive_cases [elim]: "Outj f \<turnstile> t"
 
 fun is_value :: "expr \<Rightarrow> bool" where
-  "is_value (e\<^sub>1 \<star> e\<^sub>2) = False"
+  "is_value (e\<^sub>1 \<cdot> e\<^sub>2) = False"
 | "is_value _ = True"
 
 inductive evaluate :: "expr \<Rightarrow> expr \<Rightarrow> bool" (infix "\<leadsto>" 60) where
-  ev_fun [simp]: "e\<^sub>1 \<leadsto> e\<^sub>1' \<Longrightarrow> e\<^sub>1 \<star> e\<^sub>2 \<leadsto> e\<^sub>1' \<star> e\<^sub>2"
-| ev_arg [simp]: "is_value e\<^sub>1 \<Longrightarrow> e\<^sub>2 \<leadsto> e\<^sub>2' \<Longrightarrow> e\<^sub>1 \<star> e\<^sub>2 \<leadsto> e\<^sub>1 \<star> e\<^sub>2'"
-| ev_fst [simp]: "Fst \<star> (Pair e\<^sub>1 e\<^sub>2) \<leadsto> e\<^sub>1"
-| ev_snd [simp]: "Snd \<star> (Pair e\<^sub>1 e\<^sub>2) \<leadsto> e\<^sub>2"
-| ev_csl [simp]: "Case fl fr \<star> (Inl e) \<leadsto> fl \<star> e"
-| ev_csr [simp]: "Case fl fr \<star> (Inr e) \<leadsto> fr \<star> e"
-| ev_out [simp]: "Outj f \<star> (Inj f e) \<leadsto> e"
+  ev_fun [simp]: "e\<^sub>1 \<leadsto> e\<^sub>1' \<Longrightarrow> e\<^sub>1 \<cdot> e\<^sub>2 \<leadsto> e\<^sub>1' \<cdot> e\<^sub>2"
+| ev_arg [simp]: "is_value e\<^sub>1 \<Longrightarrow> e\<^sub>2 \<leadsto> e\<^sub>2' \<Longrightarrow> e\<^sub>1 \<cdot> e\<^sub>2 \<leadsto> e\<^sub>1 \<cdot> e\<^sub>2'"
+| ev_fst [simp]: "\<pi>\<^sub>1 \<cdot> (PairV e\<^sub>1 e\<^sub>2) \<leadsto> e\<^sub>1"
+| ev_snd [simp]: "\<pi>\<^sub>2 \<cdot> (PairV e\<^sub>1 e\<^sub>2) \<leadsto> e\<^sub>2"
+| ev_tup [simp]: "f\<^sub>1 \<triangle> f\<^sub>2 \<cdot> e \<leadsto> PairV (f\<^sub>1 \<cdot> e) (f\<^sub>2 \<cdot> e)"
+| ev_inl [simp]: "\<iota>\<^sub>l \<cdot> e \<leadsto> InlV e"
+| ev_inr [simp]: "\<iota>\<^sub>r \<cdot> e \<leadsto> InrV e"
+| ev_csl [simp]: "f\<^sub>l \<nabla> f\<^sub>r \<cdot> (InlV e) \<leadsto> f\<^sub>l \<cdot> e"
+| ev_csr [simp]: "f\<^sub>l \<nabla> f\<^sub>r \<cdot> (InrV e) \<leadsto> f\<^sub>r \<cdot> e"
+| ev_out [simp]: "Outj f \<cdot> (Inj f e) \<leadsto> e"
 
 (* safety *)
 
@@ -69,12 +87,15 @@ abbreviation dne :: "expr \<Rightarrow> bool" where
   "dne e \<equiv> (\<not> (\<exists>e'. e \<leadsto> e'))"
 
 lemma [simp]: "dne UnitV" using evaluate.simps by blast
-lemma [simp]: "dne (Pair e\<^sub>1 e\<^sub>2)" using evaluate.simps by blast
-lemma [simp]: "dne Fst" using evaluate.simps by blast
-lemma [simp]: "dne Snd" using evaluate.simps by blast
-lemma [simp]: "dne (Inl e)" using evaluate.simps by blast
-lemma [simp]: "dne (Inr e)" using evaluate.simps by blast
-lemma [simp]: "dne (Case fl fr)" using evaluate.simps by blast
+lemma [simp]: "dne (PairV e\<^sub>1 e\<^sub>2)" using evaluate.simps by blast
+lemma [simp]: "dne (InlV e)" using evaluate.simps by blast
+lemma [simp]: "dne (InrV e)" using evaluate.simps by blast
+lemma [simp]: "dne \<pi>\<^sub>1" using evaluate.simps by blast
+lemma [simp]: "dne \<pi>\<^sub>2" using evaluate.simps by blast
+lemma [simp]: "dne (f\<^sub>1 \<triangle> f\<^sub>2)" using evaluate.simps by blast
+lemma [simp]: "dne \<iota>\<^sub>l" using evaluate.simps by blast
+lemma [simp]: "dne \<iota>\<^sub>r" using evaluate.simps by blast
+lemma [simp]: "dne (f\<^sub>l \<nabla> f\<^sub>r)" using evaluate.simps by blast
 lemma [simp]: "dne (Inj f e)" using evaluate.simps by blast
 lemma [simp]: "dne (Outj f)" using evaluate.simps by blast
 
@@ -96,14 +117,14 @@ theorem preservation: "e \<leadsto> e' \<Longrightarrow> e \<turnstile> t \<Long
 lemma canonical_unit: "e \<turnstile> Unit \<Longrightarrow> is_value e \<Longrightarrow> e = UnitV"
   by (induction e Unit rule: typecheck.induct) simp_all
 
-lemma canonical_prod: "e \<turnstile> Prod t\<^sub>1 t\<^sub>2 \<Longrightarrow> is_value e \<Longrightarrow> \<exists>e\<^sub>1 e\<^sub>2. e = Pair e\<^sub>1 e\<^sub>2"
+lemma canonical_prod: "e \<turnstile> t\<^sub>1 \<otimes> t\<^sub>2 \<Longrightarrow> is_value e \<Longrightarrow> \<exists>e\<^sub>1 e\<^sub>2. e = PairV e\<^sub>1 e\<^sub>2"
   by (induction e "Prod t\<^sub>1 t\<^sub>2" rule: typecheck.induct) simp_all
 
-lemma canonical_sum: "e \<turnstile> Sum t\<^sub>1 t\<^sub>2 \<Longrightarrow> is_value e \<Longrightarrow> \<exists>e'. e = Inl e' \<or> e = Inr e'"
+lemma canonical_sum: "e \<turnstile> t\<^sub>1 \<oplus> t\<^sub>2 \<Longrightarrow> is_value e \<Longrightarrow> \<exists>e'. e = InlV e' \<or> e = InrV e'"
   by (induction e "Sum t\<^sub>1 t\<^sub>2" rule: typecheck.induct) simp_all
 
-lemma canonical_mu: "e \<turnstile> Mu f \<Longrightarrow> is_value e \<Longrightarrow> \<exists>e'. e = Inj f e'"
-  by (induction e "Mu f" rule: typecheck.induct) simp_all
+lemma canonical_mu: "e \<turnstile> \<mu> f \<Longrightarrow> is_value e \<Longrightarrow> \<exists>e'. e = Inj f e'"
+  by (induction e "\<mu> f" rule: typecheck.induct) simp_all
 
 theorem progress: "e \<turnstile> t \<Longrightarrow> is_value e \<or> (\<exists>e'. e \<leadsto> e')"
   proof (induction e t rule: typecheck.induct)
@@ -117,37 +138,46 @@ theorem progress: "e \<turnstile> t \<Longrightarrow> is_value e \<or> (\<exists
             with tc_app T show ?thesis
               proof (induction e\<^sub>1 "t\<^sub>1 \<rightarrow> t\<^sub>2" arbitrary: t\<^sub>1 t\<^sub>2 rule: typecheck.induct)
               case tc_fst
-                then obtain e\<^sub>2\<^sub>1 e\<^sub>2\<^sub>2 where "e\<^sub>2 = Pair e\<^sub>2\<^sub>1 e\<^sub>2\<^sub>2" using canonical_prod by blast
-                moreover have "Fst \<star> Pair e\<^sub>2\<^sub>1 e\<^sub>2\<^sub>2 \<leadsto> e\<^sub>2\<^sub>1" by simp
+                then obtain e\<^sub>2\<^sub>1 e\<^sub>2\<^sub>2 where "e\<^sub>2 = PairV e\<^sub>2\<^sub>1 e\<^sub>2\<^sub>2" using canonical_prod by blast
+                moreover have "\<pi>\<^sub>1 \<cdot> PairV e\<^sub>2\<^sub>1 e\<^sub>2\<^sub>2 \<leadsto> e\<^sub>2\<^sub>1" by simp
                 ultimately show ?case by fastforce
               next case tc_snd
-                then obtain e\<^sub>2\<^sub>1 e\<^sub>2\<^sub>2 where "e\<^sub>2 = Pair e\<^sub>2\<^sub>1 e\<^sub>2\<^sub>2" using canonical_prod by blast
-                moreover have "Snd \<star> Pair e\<^sub>2\<^sub>1 e\<^sub>2\<^sub>2 \<leadsto> e\<^sub>2\<^sub>2" by simp
+                then obtain e\<^sub>2\<^sub>1 e\<^sub>2\<^sub>2 where "e\<^sub>2 = PairV e\<^sub>2\<^sub>1 e\<^sub>2\<^sub>2" using canonical_prod by blast
+                moreover have "\<pi>\<^sub>2 \<cdot> PairV e\<^sub>2\<^sub>1 e\<^sub>2\<^sub>2 \<leadsto> e\<^sub>2\<^sub>2" by simp
                 ultimately show ?case by fastforce
-              next case (tc_case fl t\<^sub>1 t\<^sub>3 fr t\<^sub>2)
-                then obtain e' where E: "e\<^sub>2 = Inl e' \<or> e\<^sub>2 = Inr e'" using canonical_sum by blast
+              next case (tc_tup f\<^sub>1 _ _ f\<^sub>2)
+                have "f\<^sub>1 \<triangle> f\<^sub>2 \<cdot> e\<^sub>2 \<leadsto> PairV (f\<^sub>1 \<cdot> e\<^sub>2) (f\<^sub>2 \<cdot> e\<^sub>2)" by simp
+                thus ?case by fastforce
+              next case tc_inl
+                have "\<iota>\<^sub>l \<cdot> e\<^sub>2 \<leadsto> InlV e\<^sub>2" by simp
+                thus ?case by fastforce
+              next case tc_inr
+                have "\<iota>\<^sub>r \<cdot> e\<^sub>2 \<leadsto> InrV e\<^sub>2" by simp
+                thus ?case by fastforce
+              next case (tc_case f\<^sub>l _ _ f\<^sub>r)
+                then obtain e' where E: "e\<^sub>2 = InlV e' \<or> e\<^sub>2 = InrV e'" using canonical_sum by blast
                 thus ?case
-                  proof (cases "e\<^sub>2 = Inl e'")
+                  proof (cases "e\<^sub>2 = InlV e'")
                   case True
-                    moreover have "Case fl fr \<star> Inl e' \<leadsto> fl \<star> e'" by simp
+                    moreover have "f\<^sub>l \<nabla> f\<^sub>r \<cdot> InlV e' \<leadsto> f\<^sub>l \<cdot> e'" by simp
                     ultimately show ?thesis by fastforce
                   next case False
-                    have "Case fl fr \<star> Inr e' \<leadsto> fr \<star> e'" by simp
+                    have "f\<^sub>l \<nabla> f\<^sub>r \<cdot> InrV e' \<leadsto> f\<^sub>r \<cdot> e'" by simp
                     with False E show ?thesis by fastforce
                   qed
               next case (tc_outj f)
                 then obtain e' where "e\<^sub>2 = Inj f e'" using canonical_mu by blast
-                moreover have "Outj f \<star> Inj f e' \<leadsto> e'" by simp
+                moreover have "Outj f \<cdot> Inj f e' \<leadsto> e'" by simp
                 ultimately show ?case by fastforce
               qed simp_all
           next case False
             with tc_app obtain e\<^sub>2' where "e\<^sub>2 \<leadsto> e\<^sub>2'" by blast
-            with True have "e\<^sub>1 \<star> e\<^sub>2 \<leadsto> e\<^sub>1 \<star> e\<^sub>2'" by simp
+            with True have "e\<^sub>1 \<cdot> e\<^sub>2 \<leadsto> e\<^sub>1 \<cdot> e\<^sub>2'" by simp
             thus ?thesis by auto
           qed
       next case False
         with tc_app obtain e\<^sub>1' where "e\<^sub>1 \<leadsto> e\<^sub>1'" by blast
-        hence "e\<^sub>1 \<star> e\<^sub>2 \<leadsto> e\<^sub>1' \<star> e\<^sub>2" by simp
+        hence "e\<^sub>1 \<cdot> e\<^sub>2 \<leadsto> e\<^sub>1' \<cdot> e\<^sub>2" by simp
         thus ?thesis by auto
       qed
   qed simp_all
